quarantine 8/n: SlabsCommon.fst; should pass CI
everything is ready for the actual implementation
of a quarantine mechanism

src/SlabsCommon.fst
@@ -122,6 +122,35 @@ let p_guard_unpack (#opened:_)
     (slab_vprop sc (snd b2) (fst b2))
     (is_guard sc (snd b2) (fst b2))
 
+let p_quarantine_unpack (#opened:_)
+  (sc: sc)
+  (b1 b2: blob)
+  : SteelGhost unit opened
+  ((p_quarantine sc) b1)
+  (fun _ -> slab_vprop sc (snd b2) (fst b2))
+  (requires fun _ -> b1 == b2)
+  (ensures fun h0 _ h1 ->
+    let blob1
+      : t_of (slab_vprop sc (snd b2) (fst b2))
+      = h1 (slab_vprop sc (snd b2) (fst b2)) in
+    b1 == b2 /\
+    is_quarantine sc (snd b1) (fst b1) blob1 /\
+    h0 ((p_quarantine sc) b1)
+    ==
+    h1 (slab_vprop sc (snd b2) (fst b2))
+  )
+  =
+  change_slprop_rel
+    ((p_quarantine sc) b1)
+    (slab_vprop sc (snd b2) (fst b2)
+    `VR2.vrefine`
+    is_quarantine sc (snd b2) (fst b2))
+    (fun x y -> x == y)
+    (fun _ -> ());
+  VR2.elim_vrefine
+    (slab_vprop sc (snd b2) (fst b2))
+    (is_quarantine sc (snd b2) (fst b2))
+
 let p_empty_pack (#opened:_)
   (sc: sc)
   (b1: blob)
@@ -250,6 +279,38 @@ let p_guard_pack (#opened:_)
     `VR2.vrefine`
     is_guard sc (snd b1) (fst b1))
     ((p_guard sc) b2)
+    (fun x y -> x == y)
+    (fun _ -> ())
+
+let p_quarantine_pack (#opened:_)
+  (sc: sc)
+  (b1: blob)
+  (b2: blob)
+  : SteelGhost unit opened
+  (slab_vprop sc (snd b1) (fst b1))
+  (fun _ -> (p_quarantine sc) b2)
+  (requires fun h0 ->
+    let blob0
+      : t_of (slab_vprop sc (snd b1) (fst b1))
+      = h0 (slab_vprop sc (snd b1) (fst b1)) in
+    is_quarantine sc (snd b1) (fst b1) blob0 /\
+    b1 == b2
+  )
+  (ensures fun h0 _ h1 ->
+    b1 == b2 /\
+    h1 ((p_quarantine sc) b2)
+    ==
+    h0 (slab_vprop sc (snd b1) (fst b1))
+  )
+  =
+  VR2.intro_vrefine
+    (slab_vprop sc (snd b1) (fst b1))
+    (is_quarantine sc (snd b1) (fst b1));
+  change_slprop_rel
+    (slab_vprop sc (snd b1) (fst b1)
+    `VR2.vrefine`
+    is_quarantine sc (snd b1) (fst b1))
+    ((p_quarantine sc) b2)
     (fun x y -> x == y)
     (fun _ -> ())
 #pop-options
@@ -393,10 +454,10 @@ let pack_3
   (md_bm_region: array U64.t{A.length md_bm_region = US.v metadata_max * 4})
   (md_region: array AL.cell{A.length md_region = US.v metadata_max})
   (md_count: ref US.t)
-  (r1 r2 r3 r4: ref US.t)
+  (r1 r2 r3 r4 r5: ref US.t)
   (md_count_v: US.t{US.v md_count_v <= US.v metadata_max})
   (md_region_lv: G.erased (Seq.lseq AL.status (US.v md_count_v)))
-  (idx1 idx2 idx3 idx4: US.t)
+  (idx1 idx2 idx3 idx4 idx5: US.t)
   : SteelGhost unit opened
   (
     vptr md_count `star`
@@ -404,9 +465,10 @@ let pack_3
     vptr r2 `star`
     vptr r3 `star`
     vptr r4 `star`
-    (AL.varraylist pred1 pred2 pred3 pred4
+    vptr r5 `star`
+    (AL.varraylist pred1 pred2 pred3 pred4 pred5
       (A.split_l md_region md_count_v)
-      (US.v idx1) (US.v idx2) (US.v idx3) (US.v idx4)) `star`
+      (US.v idx1) (US.v idx2) (US.v idx3) (US.v idx4) (US.v idx5)) `star`
     starseq
       #(pos:US.t{US.v pos < US.v md_count_v})
       #(t size_class)
@@ -418,41 +480,44 @@ let pack_3
     vrefinedep
       (vptr md_count)
       vrefinedep_prop
-      (left_vprop size_class slab_region md_bm_region md_region r1 r2 r3 r4)
+      (left_vprop size_class slab_region md_bm_region md_region r1 r2 r3 r4 r5)
   )
   (requires fun h0 ->
-    let gs0 = AL.v_arraylist pred1 pred2 pred3 pred4
+    let gs0 = AL.v_arraylist pred1 pred2 pred3 pred4 pred5
       (A.split_l md_region md_count_v)
-      (US.v idx1) (US.v idx2) (US.v idx3) (US.v idx4) h0 in
+      (US.v idx1) (US.v idx2) (US.v idx3) (US.v idx4) (US.v idx5) h0 in
     US.v md_count_v <> AL.null /\
     sel md_count h0 == md_count_v /\
     sel r1 h0 == idx1 /\
     sel r2 h0 == idx2 /\
     sel r3 h0 == idx3 /\
     sel r4 h0 == idx4 /\
+    sel r5 h0 == idx5 /\
     ALG.dataify gs0 `Seq.equal` G.reveal md_region_lv /\
-    ALG.partition #AL.status gs0 (US.v idx1) (US.v idx2) (US.v idx3) (US.v idx4)
+    ALG.partition #AL.status gs0 (US.v idx1) (US.v idx2) (US.v idx3) (US.v idx4) (US.v idx5)
   )
   (ensures fun _ _ h1 ->
     let blob1
       = h1 (vrefinedep
       (vptr md_count)
       vrefinedep_prop
-      (left_vprop size_class slab_region md_bm_region md_region r1 r2 r3 r4)
+      (left_vprop size_class slab_region md_bm_region md_region r1 r2 r3 r4 r5)
     ) in
     md_count_v == dfst blob1)
   =
   intro_vrefine
-    (ind_varraylist_aux2 pred1 pred2 pred3 pred4
-      (A.split_l md_region md_count_v) (((idx1, idx2), idx3), idx4))
-    (ind_varraylist_aux_refinement pred1 pred2 pred3 pred4
-      (A.split_l md_region md_count_v) (((idx1, idx2), idx3), idx4));
-  intro_vdep
-    (vptr r1 `star` vptr r2 `star` vptr r3 `star` vptr r4)
-    (ind_varraylist_aux pred1 pred2 pred3 pred4
+    (ind_varraylist_aux2
       (A.split_l md_region md_count_v)
-      (((idx1, idx2), idx3), idx4))
-    (ind_varraylist_aux pred1 pred2 pred3 pred4
+      ((((idx1, idx2), idx3), idx4), idx5))
+    (ind_varraylist_aux_refinement
+      (A.split_l md_region md_count_v)
+      ((((idx1, idx2), idx3), idx4), idx5));
+  intro_vdep
+    (vptr r1 `star` vptr r2 `star` vptr r3 `star` vptr r4 `star` vptr r5)
+    (ind_varraylist_aux
+      (A.split_l md_region md_count_v)
+      ((((idx1, idx2), idx3), idx4), idx5))
+    (ind_varraylist_aux
       (A.split_l md_region md_count_v));
 
   change_equal_slprop
@@ -465,15 +530,15 @@ let pack_3
     (left_vprop2 size_class slab_region md_bm_region md_count_v (G.reveal md_region_lv));
 
   intro_vdep
-    (left_vprop1 md_region r1 r2 r3 r4 md_count_v)
+    (left_vprop1 md_region r1 r2 r3 r4 r5 md_count_v)
     (left_vprop2 size_class slab_region md_bm_region md_count_v (G.reveal md_region_lv))
-    (left_vprop_aux size_class slab_region md_bm_region md_region r1 r2 r3 r4 md_count_v);
+    (left_vprop_aux size_class slab_region md_bm_region md_region r1 r2 r3 r4 r5 md_count_v);
 
   intro_vrefinedep
     (vptr md_count)
     vrefinedep_prop
-    (left_vprop size_class slab_region md_bm_region md_region r1 r2 r3 r4)
-    (left_vprop size_class slab_region md_bm_region md_region r1 r2 r3 r4 md_count_v)
+    (left_vprop size_class slab_region md_bm_region md_region r1 r2 r3 r4 r5)
+    (left_vprop size_class slab_region md_bm_region md_region r1 r2 r3 r4 r5 md_count_v)
 #pop-options
 
 let lemma_slab_aux_starseq
@@ -511,7 +576,7 @@ let pack_slab_starseq
   (md_bm_region: array U64.t{A.length md_bm_region = US.v metadata_max * 4})
   (md_region: array AL.cell{A.length md_region = US.v metadata_max})
   (md_count: ref US.t)
-  (r1 r2 r3 r4: ref US.t)
+  //(r1 r2 r3 r4 r5: ref US.t)
   (md_count_v: US.t{US.v md_count_v <= US.v metadata_max})
   (md_region_lv: G.erased (Seq.lseq AL.status (US.v md_count_v)))
   (idx: US.t{US.v idx < US.v md_count_v})
@@ -550,6 +615,9 @@ let pack_slab_starseq
       (slab_array slab_region idx)
       (md_bm_array md_bm_region idx)) in
     let md : Seq.lseq U64.t 4 = dfst md_blob in
+    (v == 4ul ==> is_quarantine size_class
+      (slab_array slab_region idx)
+      (md_bm_array md_bm_region idx) md_blob) /\
     (v == 3ul ==> is_guard size_class
       (slab_array slab_region idx)
       (md_bm_array md_bm_region idx) md_blob) /\
@@ -561,7 +629,17 @@ let pack_slab_starseq
   (ensures fun h0 _ h1 -> True)
   =
   SeqUtils.init_us_refined_index (US.v md_count_v) (US.v idx);
-  if U32.eq v 3ul then (
+  if (U32.eq v 4ul) then (
+    p_quarantine_pack size_class
+      (md_bm_array md_bm_region idx,
+      slab_array slab_region idx)
+      (md_bm_array md_bm_region idx,
+      slab_array slab_region idx);
+    change_equal_slprop
+      (p_quarantine size_class (md_bm_array md_bm_region idx, slab_array slab_region idx))
+      (f size_class slab_region md_bm_region md_count_v (Seq.upd md_region_lv (US.v idx) v)
+        (Seq.index (SeqUtils.init_us_refined (US.v md_count_v)) (US.v idx)))
+  ) else if (U32.eq v 3ul) then (
     p_guard_pack size_class
       (md_bm_array md_bm_region idx,
       slab_array slab_region idx)
@@ -571,7 +649,7 @@ let pack_slab_starseq
       (p_guard size_class (md_bm_array md_bm_region idx, slab_array slab_region idx))
       (f size_class slab_region md_bm_region md_count_v (Seq.upd md_region_lv (US.v idx) v)
         (Seq.index (SeqUtils.init_us_refined (US.v md_count_v)) (US.v idx)))
-  ) else if U32.eq v 2ul then (
+  ) else if (U32.eq v 2ul) then (
     p_full_pack size_class
       (md_bm_array md_bm_region idx,
       slab_array slab_region idx)
@@ -581,7 +659,7 @@ let pack_slab_starseq
       (p_full size_class (md_bm_array md_bm_region idx, slab_array slab_region idx))
       (f size_class slab_region md_bm_region md_count_v (Seq.upd md_region_lv (US.v idx) v)
         (Seq.index (SeqUtils.init_us_refined (US.v md_count_v)) (US.v idx)))
-  ) else if U32.eq v 1ul then (
+  ) else if (U32.eq v 1ul) then (
     p_partial_pack size_class
       (md_bm_array md_bm_region idx,
       slab_array slab_region idx)
@@ -592,7 +670,7 @@ let pack_slab_starseq
       (f size_class slab_region md_bm_region md_count_v (Seq.upd md_region_lv (US.v idx) v)
         (Seq.index (SeqUtils.init_us_refined (US.v md_count_v)) (US.v idx)))
   ) else (
-     p_empty_pack size_class
+    p_empty_pack size_class
       (md_bm_array md_bm_region idx,
       slab_array slab_region idx)
       (md_bm_array md_bm_region idx,
@@ -626,14 +704,14 @@ let pack_right_and_refactor_vrefine_dep
   (md_bm_region: array U64.t{A.length md_bm_region = US.v metadata_max * 4})
   (md_region: array AL.cell{A.length md_region = US.v metadata_max})
   (md_count: ref US.t)
-  (r1 r2 r3 r4: ref US.t)
+  (r1 r2 r3 r4 r5: ref US.t)
   (md_count_v: US.t{US.v md_count_v <= US.v metadata_max})
   : SteelGhost unit opened
   (
     vrefinedep
       (vptr md_count)
       vrefinedep_prop
-      (left_vprop size_class slab_region md_bm_region md_region r1 r2 r3 r4)
+      (left_vprop size_class slab_region md_bm_region md_region r1 r2 r3 r4 r5)
     `star`
     right_vprop slab_region md_bm_region md_region md_count_v
   )
@@ -641,14 +719,14 @@ let pack_right_and_refactor_vrefine_dep
     vrefinedep
       (vptr md_count)
       vrefinedep_prop
-      (size_class_vprop_aux size_class slab_region md_bm_region md_region r1 r2 r3 r4)
+      (size_class_vprop_aux size_class slab_region md_bm_region md_region r1 r2 r3 r4 r5)
   )
   (requires fun h0 ->
     let blob0
       = h0 (vrefinedep
       (vptr md_count)
       vrefinedep_prop
-      (left_vprop size_class slab_region md_bm_region md_region r1 r2 r3 r4)
+      (left_vprop size_class slab_region md_bm_region md_region r1 r2 r3 r4 r5)
     ) in
     md_count_v == dfst blob0)
   (ensures fun h0 _ h1 ->
@@ -656,13 +734,13 @@ let pack_right_and_refactor_vrefine_dep
       = h0 (vrefinedep
       (vptr md_count)
       vrefinedep_prop
-      (left_vprop size_class slab_region md_bm_region md_region r1 r2 r3 r4)
+      (left_vprop size_class slab_region md_bm_region md_region r1 r2 r3 r4 r5)
     ) in
     let blob1
       = h1 (vrefinedep
       (vptr md_count)
       vrefinedep_prop
-      (size_class_vprop_aux size_class slab_region md_bm_region md_region r1 r2 r3 r4)
+      (size_class_vprop_aux size_class slab_region md_bm_region md_region r1 r2 r3 r4 r5)
     ) in
     dfst blob0 == dfst blob1
   )
@@ -670,7 +748,7 @@ let pack_right_and_refactor_vrefine_dep
   let md_count_v' = elim_vrefinedep
     (vptr md_count)
     vrefinedep_prop
-    (left_vprop size_class slab_region md_bm_region md_region r1 r2 r3 r4) in
+    (left_vprop size_class slab_region md_bm_region md_region r1 r2 r3 r4 r5) in
   assert (G.reveal md_count_v' == md_count_v);
   change_equal_slprop
     (right_vprop slab_region md_bm_region md_region md_count_v)
@@ -679,7 +757,7 @@ let pack_right_and_refactor_vrefine_dep
   intro_vrefinedep
     (vptr md_count)
     vrefinedep_prop
-    (size_class_vprop_aux size_class slab_region md_bm_region md_region r1 r2 r3 r4)
-    (left_vprop size_class slab_region md_bm_region md_region r1 r2 r3 r4 (G.reveal md_count_v') `star`
+    (size_class_vprop_aux size_class slab_region md_bm_region md_region r1 r2 r3 r4 r5)
+    (left_vprop size_class slab_region md_bm_region md_region r1 r2 r3 r4 r5 (G.reveal md_count_v') `star`
     right_vprop slab_region md_bm_region md_region (G.reveal md_count_v'))
 #pop-options
